src/program_proof/tulip/invariance/execute_commit.v
@@ -8,12 +8,12 @@ Section execute_commit.
     let clog' := clog ++ [CmdCommit ts pwrs] in
     Forall (λ nc, (nc.1 <= length clog)%nat) ilog ->
     is_txn_log_lb γ gid clog' -∗
-    own_replica_clog_half γ rid clog -∗
-    own_replica_ilog_half γ rid ilog -∗
+    own_replica_clog_half γ gid rid clog -∗
+    own_replica_ilog_half γ gid rid ilog -∗
     group_inv γ gid -∗
     replica_inv γ gid rid ==∗
-    own_replica_clog_half γ rid clog' ∗
-    own_replica_ilog_half γ rid ilog ∗
+    own_replica_clog_half γ gid rid clog' ∗
+    own_replica_ilog_half γ gid rid ilog ∗
     group_inv γ gid ∗
     replica_inv γ gid rid.
   Proof.
